WSC/Prep/Minting800.lean
@@ -1,0 +1,14 @@
+import PlutusCore.UPLC
+import CardanoLedgerApi.V3
+import Blaster
+namespace WSC
+open CardanoLedgerApi.IsData.Class (toTerm)
+open CardanoLedgerApi.V3 (ScriptContext CurrencySymbol ScriptHash mintingInputs)
+open PlutusCore.UPLC.Term (Term)
+set_option maxHeartbeats 0
+#import_uplc programmableTokenMinting800 PlutusV3 double_cbor_hex "WSC/flats/programmableTokenMinting.flat"
+def mintingPolicyInputs800 (protocolParamsCS : CurrencySymbol) (mintingLogicHash : ScriptHash)
+    (ctx : ScriptContext) : List Term :=
+  toTerm protocolParamsCS :: toTerm mintingLogicHash :: mintingInputs ctx
+#prep_uplc appliedMinting800 programmableTokenMinting800 mintingPolicyInputs800 800
+end WSC
